completeness base case

lemma/completeness.v
@@ -11,13 +11,17 @@ From Coq Require Import IndefiniteDescription.
 
 Import ListNotations.
 
-(*
-Lemma lem_simul_assoc_inv: assoc gamma g ->
-    M.find p gamma = Some (ltt_send q xsp) ->
-    M.find q gamma = Some (ltt_recv p xsq) ->
-    (exists gcs, g= gtt_send p q gcs) \/
-    ()
-*)
+
+Ltac tac_use_assoc Hassoc p Hisparts := 
+    let Ha1:=fresh "Hassoc" in let Ha2:=fresh "Hassoc" in 
+    let Ha3:=fresh "Hassoc" in
+    pose proof Hassoc as Ha3;
+    unfold assoc in Ha3;
+specialize (Ha3 p); 
+    destruct Ha3 as [Ha1 Ha2];
+    let Har:=fresh "Hassoc_u" in 
+try (specialize (Ha1 Hisparts) as Har;clear Ha2 Ha1);try (specialize (Ha2 Hisparts) as Har;clear Ha1 Ha2).
+
 
 Section AssocCompletenessHelpers.
 Variables (gamma: tctx) (g:gtt).
@@ -38,16 +42,6 @@ Proof.
 Qed.
 Check Proper.
 
-
-Ltac tac_use_assoc Hassoc p Hisparts := 
-    let Ha1:=fresh "Hassoc" in let Ha2:=fresh "Hassoc" in 
-    let Ha3:=fresh "Hassoc" in
-    pose proof Hassoc as Ha3;
-    unfold assoc in Ha3;
-specialize (Ha3 p); 
-    destruct Ha3 as [Ha1 Ha2];
-    let Har:=fresh "Hassoc_u" in 
-try (specialize (Ha1 Hisparts) as Har;clear Ha2 Ha1);try (specialize (Ha2 Hisparts) as Har;clear Ha1 Ha2).
 
 
 Lemma assoc_weakening: forall p, (~ isgPartsC p g) 
@@ -154,47 +148,370 @@ Proof. unfold "==>"; red; intros;subst; split;intros; [ | symmetry in H];
 eapply assoc_m with (g:=y0) in H;try easy.
 Qed.
 
+Definition partial_assoc (gamma:tctx) (g:gtt) :=
+    forall p Tp, M.find p gamma = Some Tp -> issubProj Tp g p.
+(*assoc = largest partial assoc*)
+
+Lemma partial_assoc_strengthening: forall gamma p Tp g, wfgC g ->
+M.find p gamma = None ->
+partial_assoc (M.add p Tp gamma) g -> partial_assoc gamma g.
+Proof.
+    red. intros * Hwfg Hnone Hassoc. red in Hassoc. intros. specialize (Hassoc p0 Tp0).
+    destruct (Nat.eq_dec p p0);subst; autorewrite with mmaps in Hassoc;crush.
+Qed.
+
+Lemma assoc_is_partial_assoc : forall gamma g,
+wfgC g -> assoc gamma g -> partial_assoc gamma g.
+Proof.
+    intros * Hwfg Hassoc. red;intros. 
+    specialize (Hassoc p). destruct (decidable_isgPartsC g p);try easy.
+    {
+        destr_hyps. specialize (H1 H0). crush.   
+    }
+    {
+        destr_hyps. specialize (H2 H0 Tp). crush. red. exists ltt_end.
+        split;[apply not_part_proj;easy|apply stRefl].   
+    }
+Qed.
+
+Lemma assoc_to_partial_assoc_add : forall gamma p Tp g,
+wfgC g->
+M.find p gamma = None -> 
+assoc (M.add p Tp gamma) g -> partial_assoc gamma g.
+Proof.
+    red. intros * Hwfg Hnone Hassoc *. red in Hassoc. specialize (Hassoc p0).
+    destr_hyps. 
+    destruct (decidable_isgPartsC  g p0);try easy.
+    apply H in H1. destr_hyps. intros.
+    destruct (Nat.eq_dec p p0);subst;autorewrite with mmaps in *;crush.
+    intros.
+    destruct (Nat.eq_dec p p0);subst;autorewrite with mmaps in *;crush.
+    eapply H3 in H2;subst. red. exists ltt_end. split.
+    apply not_part_proj;easy. apply stRefl.
+Qed. 
+
+Lemma partial_assoc_to_assoc : forall gamma g, wfgC g ->
+partial_assoc gamma g -> (forall p, isgPartsC p g -> M.In p gamma) ->
+assoc gamma g.
+Proof.
+    intros * Hwfg Hpassoc Hsubset.
+    red. intros;split;intros.
+    {
+        red in Hpassoc.
+        specialize (Hsubset p H). rewrite MF.in_find in Hsubset. apply opt_lem1 in Hsubset. destr_hyps.
+        exists x. specialize (Hpassoc p x H0). easy.   
+    }
+    {
+        red in Hpassoc.
+        specialize (Hpassoc p Tpx H0). apply not_part_proj in H. red in Hpassoc. destr_hyps.
+        eapply proj_inj in H;try exact H1;try easy;subst. apply subtype_end_inv in H2. easy.   
+    }
+Qed.
+
+Lemma part_after_step_redux : forall g g' p q ell r, wfgC g -> projectableA g -> gttstepC g g' p q ell -> isgPartsC r g' 
+-> isgPartsC r g.
+Proof.
+    intros.
+    Search isgPartsC gttstepC.
+    pose proof H1 as Hstep. eapply proj_cont_pq_step in Hstep;try easy.
+    destr_hyps.
+    eapply part_after_step with (G':=g') (q:=p) (p:=q) (l:=ell) (LP:=x) (LQ:=x0);try easy.
+    
+    eapply wfgC_after_step in H1;easy.
+Qed.
+
+#[export] Instance PASSMEQ {A: Type}: Proper (M.Equal ==> eq ==> (iff)) partial_assoc.
+Proof. unfold "==>"; red; intros;subst; split;intros; [ | symmetry in H]; 
+    red; intros; red in H0; specialize (H0 p Tp); apply H0;
+    red in H; crush.    
+Qed.
+
+Lemma partial_assoc_extend: forall gamma g p T, partial_assoc gamma g -> M.find p gamma =None -> issubProj T g p -> 
+partial_assoc (M.add p T gamma) g.
+Proof. 
+    intros * Hpassoc Hnone Hsubproj; red;intros;
+    destruct (Nat.eq_dec p p0);subst; autorewrite with mmaps in H;crush.
+Qed. 
+
+Lemma partial_assoc_inv_send: forall p q xs gamma G,
+wfgC G ->
+SList xs ->
+partial_assoc gamma G ->
+M.find p gamma =Some  (ltt_send q xs)  ->
+(exists ys : list (option (sort * gtt)), G = gtt_send p q ys /\ send_cond xs ys p) \/
+(exists (s t : opt_lbl) (ys : list (option (sort * gtt))),
+G = gtt_send s t ys /\ p <> s /\ p <> t /\ subproj_cont_cond (ltt_send q xs) ys p).
+Proof.
+    intros.
+    pose proof H as Hwfg.
+    apply decidable_isgPartsC with (pt:= p) in H.
+    specialize (H1 p).
+    
+    destr_hyps.
+    destruct H.
+    eapply H1 in H2.
+    apply subproj_inv_send in H2;crush.
+    specialize (H1 _ H2).
+    red in H1. destr_hyps. apply not_part_proj in H. 
+    eapply proj_inj with (t:=ltt_end)in H1;try easy;subst.
+    pinversion H3;apply sub_mon.
+Qed.
+
+Lemma partial_assoc_inv_recv: forall p q xs gamma G,
+wfgC G ->
+SList xs ->
+partial_assoc gamma G ->
+M.find p gamma =Some  (ltt_recv q xs)  ->(exists ys : list (option (sort * gtt)),
+G = gtt_send q p ys /\ recv_cond xs ys p) \/
+(exists (s t : opt_lbl) (ys : list (option (sort * gtt))),
+G = gtt_send s t ys /\
+p <> s /\ p <> t /\ subproj_cont_cond (ltt_recv q xs) ys p).
+Proof.
+    intros.
+    pose proof H as Hwfg.
+    apply decidable_isgPartsC with (pt:= p) in H.
+    specialize (H1 p).
+    
+    destr_hyps.
+    destruct H.
+    eapply H1 in H2.
+    apply subproj_inv_recv in H2;crush.
+    specialize (H1 _ H2).
+    red in H1. destr_hyps. apply not_part_proj in H. 
+    eapply proj_inj with (t:=ltt_end)in H1;try easy;subst.
+    pinversion H3;apply sub_mon.
+Qed.
+
+Lemma partial_assoc_simul_inv: 
+    forall gamma g p q xp xq, 
+    tctx_wf gamma ->
+    wfgC g ->
+    partial_assoc gamma g ->
+    M.find p gamma = Some (ltt_send q xp) -> 
+    M.find q gamma = Some (ltt_recv p xq) ->
+    (
+        exists xg, g=gtt_send p q xg /\
+        send_cond xp xg p  /\
+        recv_cond
+        xq xg q
+    )
+    \/
+    (
+        exists s t xg, g=gtt_send s t xg /\
+        p <> s /\ q <> t /\ 
+        Forall (fun u=> u=None \/ exists s g, u=Some (s,g) /\ issubProj (ltt_send q xp) g p
+        /\ issubProj (ltt_recv p xq) g q
+        ) xg
+    )
+    .
+Proof.
+    intros * Htctx_wf Hwfg Hassoc Hfindp Hfindq.
+    
+    tac_tctx_wf_to_slist xp Htctx_wf Hfindp q.
+    tac_tctx_wf_to_slist xq Htctx_wf Hfindq p.
+    eapply  partial_assoc_inv_send with (G:=g) in Hfindp;try easy.
+    eapply  partial_assoc_inv_recv with (G:=g) in Hfindq; try easy.
+    destruct Hfindp;destruct Hfindq;crush.
+    {
+
+        left.
+        exists x0. crush. 
+        (*follows from the assumptions*)    
+    }
+    {
+        right. rename x2 into s, x3 into t, x4 into xg. 
+        exists s, t, xg. crush.
+        eapply Forall_forall.
+        intros.
+        destruct x2;crush.
+        right.
+        destruct p0 as [s0 g].
+        exists s0, g.
+        Check Forall_forall.
+        Search In onth.
+        apply in_some_implies_onth in H7. destruct H7 as [n].
+        split;try easy.   
+        unfold subproj_cont_cond in H6, H8.
+        inversion H3;subst;clear H3.
+        split;
+        [eapply Forall_prop with (l:=n) (p:=(s0,g)) in H8 |
+        eapply Forall_prop with (l:=n) (p:=(s0,g)) in H6]; crush.
+    }
+Qed.
+Lemma subproj_after_cont_wfltt: forall p q r gcs s gk Tp k,
+    wflttC Tp ->
+    wfgC (gtt_send p q gcs) ->
+    issubProj Tp (gtt_send p q gcs) r -> 
+    r <> p -> r<> q ->
+    onth k gcs=Some (s,gk) -> issubProj Tp gk r.
+Proof.
+    intros.
+    destruct (decidable_isgPartsC (gtt_send p q gcs) r);try easy.
+    destruct Tp;
+    [eapply subproj_inv_end in H1
+    | apply wfltt_slist_recv in H; 
+    eapply subproj_after_cont_recv with (p:=p) (q:=q) (gcs:=gcs) (k:=k) (s:=s)
+    |apply wfltt_slist_send in H; 
+    eapply subproj_after_cont_send with (p:=p) (q:=q) (gcs:=gcs) (k:=k) (s:=s)]; try easy.
+    assert(isgPartsC r gk -> False) by 
+    (intros; eapply part_parent with (k:=k) (gcs:=gcs) (p:=p) (q:=q) (s:=s) in H6;
+    try easy).
+    red in H1. destr_hyps. apply not_part_proj in H5. 
+    eapply proj_inj with (t:=x) in H5;try easy;subst.
+    apply subtype_end_inv in H7;subst.
+    apply not_part_proj in H6. exists ltt_end. split;try easy;try apply stRefl.
+Qed.
+
+Theorem assoc_completeness' : forall p q ell gamma gamma' g, partial_assoc gamma g ->
+wfgC g -> projectableA g -> tctx_wf gamma ->
+tctxR gamma (lcomm p q ell) gamma' ->
+exists g', partial_assoc gamma' g' /\ gttstepC g g' p q ell. 
+Proof.
+    intros * Hassoc Hwfg Hproj Hwfltt Hred.
+    assert (exists xsp, M.find p  gamma = Some (ltt_send q xsp)).
+    {
+        eapply lem_6_11c_tctx_comm_invert in Hred. destr_hyps. exists x1. easy.   
+    }
+    assert (exists xsq, M.find q  gamma = Some (ltt_recv p xsq)).
+    {
+        eapply lem_6_11c_tctx_comm_invert in Hred. destr_hyps. exists x4. easy.   
+    }
+    dependent induction Hred.
+    {
+        rename H1 into Hdisj1, H2 into Hdisj2.
+        destruct H3 as [xsp Hfindp].
+        destruct H4 as [xsq Hfindq].
+        pose proof Hassoc as Hsimul.
+        eapply partial_assoc_simul_inv with (p:=p) (q:=q) (xp:=xsp) (xq:=xsq) in Hsimul;try easy.
+        destruct Hsimul.
+        {
+            destruct H1 as [xg [H1 [Hsendcond Hreccond]]]. subst.
+            red in Hsendcond.
+            pose proof Hwfltt as Hslistxp.
+            set (comb:=disj_merge g1 g2 Hdisj1).
+            red in Hslistxp. specialize (Hslistxp p (ltt_send q xsp) Hfindp).
+            apply wfltt_slist_send in Hslistxp.
+            assert(exists sk gk,onth ell xg = Some (sk, gk)).
+            {
+                apply lem_6_11a_tctx_send_invert in Hred1.
+                destruct Hred1 as [xsp' [Tp' Hred1]].
+                destr_hyps.
+                eapply spc_merge_find1 with (g2:=g2) (H_disj:=Hdisj1) in H1.
+                rewrite Hfindp in H1.
+                inversion H1;subst.
+                eapply Forall2R_prop with (l:=ell) (p:=(s,Tp')) in Hsendcond;try easy.
+                destruct Hsendcond as [p' [Honth Hsend]].
+                destruct Hsend;try easy.
+                destr_hyps.
+                inversion H2;subst.
+                clear H2.
+                rename x1 into sk,x2 into gk, x into s1, x0 into T1.
+                exists sk, gk. easy.
+            }
+            destruct H1 as [sk [gk Honthxg]].
+            assert (Hnstep:gttstepC (gtt_send p q xg) gk p q ell).
+            {
+                pfold. econstructor;try easy. symmetry in  Honthxg. exact Honthxg.
+            }
+            exists gk.
+            split;try easy.
+            red. intros.
+            destruct (Nat.eq_dec p0 p);
+            destruct (Nat.eq_dec p0 q);subst;try easy.
+            {
+                
+                apply lem_6_11a_tctx_send_invert in Hred1.
+                move Hred1 at bottom.
+                destr_hyps.
+                eapply spc_merge_find1 with (g2:=g2) (H_disj:=Hdisj1) in H2.
+                rewrite Hfindp in H2.
+                symmetry in H2;inversion H2;subst. clear H2.
+                eapply Forall2R_prop with (l:=ell) (p:=(s,x0)) in Hsendcond;try easy.
+                move Hsendcond at bottom.
+                destr_hyps.
+                destruct H5;try easy;destr_hyps.
+                eapply spc_merge_find1 with (g2:=g2') (H_disj:=Hdisj2) in H4. crush.
+            }
+            {
+                apply lem_6_11b_tctx_recv_invert in Hred2.
+                move Hred2 at bottom.
+                destr_hyps.
+                eapply spc_merge_find2 with (g1:=g1) (H_disj:=Hdisj1) in H2.
+                rewrite Hfindq in H2.
+                symmetry in H2;inversion H2;subst. clear H2.
+                eapply Forall2R_prop with (l:=ell) (p:=(sk,gk)) in Hreccond;try easy.
+                
+                destr_hyps.
+                destruct H5;try easy;destr_hyps.
+                eapply spc_merge_find2 with (g1:=g1') (H_disj:=Hdisj2) in H4. crush.
+            }
+            {
+                Search p0.
+                Search tctxR M.find.   
+                assert(Har:tctxR (disj_merge g1 g2 Hdisj1) (lcomm p q ell) (disj_merge g1' g2' Hdisj2)).
+                {
+                    econstructor;try easy. exact Hred1. exact Hred2. exact H0.   
+                }
+                eapply lem_6_10 with (r:=p0) in Har.
+                rewrite <- Har in H1.
+                move Hassoc at bottom. red in Hassoc. specialize (Hassoc p0 Tp H1).
+                eapply subproj_after_cont_wfltt with (p:=p) (q:=q) (gcs:=xg) (k:=ell) (s:=sk);try easy.
+                specialize (Hwfltt p0). apply Hwfltt;easy.
+                crush.
+            }
+        }
+    }
+    {
+        rename g0 into gamma, g' into gamma'.
+        rewrite MF.not_mem_find in H.
+        apply lem_6_11c_tctx_comm_invert in Hred. destr_hyps.
+        destruct (Nat.eq_dec p0 p);destruct (Nat.eq_dec p0 q);crush.
+        rename x into s, x0 into s', x3 into xsq, x1 into xsp, x2 into Tp, x4 into Tq.
+        assert (Hpassoc:partial_assoc gamma g) by admit.
+        assert (Hwf2: tctx_wf gamma) by admit.
+        eapply IHHred with (p:=p) (q:=q) (ell:=ell) in Hpassoc;try easy.
+        
+        destr_hyps.
+        exists x.
+        split;try easy.
+        apply partial_assoc_extend;try easy.
+        admit. (*by eqdom*)
+        Search T.
+        pose proof Hassoc as Hassocb.
+        red in Hassoc. specialize (Hassoc p0 T).
+        autorewrite with mmaps in Hassoc. specialize (Hassoc (eq_refl _ )).
+        Search gttstepC issubProj.
+        eapply subproj_after_step_r with (r:=p0) (x:=T) in H8;try easy.
+        apply wfgC_after_step in H8;try easy.
+    }
+    {
+        admit.   
+    }
+Admitted.
 Theorem assoc_completeness: forall p q ell gamma gamma' g, assoc gamma g ->
     wfgC g ->
+    tctx_wf gamma ->
     tctxR gamma (lcomm p q ell) gamma' ->
     exists g', assoc gamma' g' /\ gttstepC g g' p q ell.
 Proof.
-    intros * Hassoc Hwfg Hred.
-    dependent induction Hred.
+    intros * Hassoc Hwfg Hwfltt Hred.
+    pose proof Hred as Heqdom.
+    pose proof Hassoc as Ha1.
+    eapply assoc_is_partial_assoc in Hassoc;try easy. 
+    eapply assoc_completeness' with (g:=g) in Hred;try easy.
+    destr_hyps.
+    exists x.
+    split;try easy.
+    eapply partial_assoc_to_assoc;try easy.
+    apply wfgC_after_step in H0;try easy. apply assoc_implies_projectable in Ha1;try easy.
+    
+    intros.
+    assert (isgPartsC p0 g).
     {
-        clear IHHred1 IHHred2.
-        rename H1 into Hdisj1, H2 into Hdisj2.
-        admit.
+        eapply part_after_step_redux with (r:=p0)in H0;try easy.
+        apply assoc_implies_projectable in Ha1;try easy.   
     }
-    {   
-        rename g0 into gamma, g' into gamma'.
-        destruct T.
-        
-        rewrite MF.not_mem_find in H.
-        (*t must be ltt end*)
-        {
-            assert (Hassoc_gamma: assoc gamma g).
-            {
-                eapply assoc_remove_end with (p:=p0) in Hassoc;try (autorewrite with mmaps;easy).
-                (*follows by setoid rewrite*)
-                admit.   
-            }
-            eapply assoc_remove_end with (p:=p0)in Hassoc;try (autorewrite with mmaps;easy).
-            
-            eapply assoc_context_not_in_global_not_in with (g:=g) in H;try easy.
-            pose proof Hwfg.
-            eapply IHHred with (p:=p) (q:=q) (ell:=ell) in H0;try easy.
-            destr_hyps.
-            exists x.
-            split;try easy.
-            eapply assoc_weakening;try easy.
-            
-            eapply not_part_step with (g:=g) (p:=p) (q:=q) (k:=ell);try easy.
-            eapply assoc_implies_projectable with (gamma:=gamma);try easy.
-        }
-        {
-            
-        }
-        exists g0.
-        admit.
-    }
+    eapply dom_preservation_6_9 in Heqdom.
+    tac_use_assoc Ha1 p0 H2. destr_hyps. apply opt_lem2 in H3. rewrite  <- MF.in_find in H3.
+    apply Heqdom in H3. easy.
+Qed.
